use meaningful name.

src/dafny/beacon/attestations/AttestationsHelpers.dfy
@@ -210,17 +210,17 @@ module AttestationsHelpers {
         ensures var e := get_previous_epoch(state);
             epoch == e ==> 
                 get_matching_target_attestations(state, e) == 
-                filterAttestationsxx(state.previous_epoch_attestations, get_block_root(state, e))
+                filterAttestations(state.previous_epoch_attestations, get_block_root(state, e))
         ensures var e := get_current_epoch(state);
             epoch == e ==> 
                 get_matching_target_attestations(state, e) == 
-                filterAttestationsxx(state.current_epoch_attestations, get_block_root(state, e))
+                filterAttestations(state.current_epoch_attestations, get_block_root(state, e))
         decreases epoch //  seems needed to prove last two post-conds
     {
         //  Get attestattions at epoch as recorded in state (previous epoch or current epoch).
         var ax := get_matching_source_attestations(state, epoch);
         //  Collect attestations for (i.e. with target equal to) block root at epoch
-        filterAttestationsxx(ax, get_block_root(state, epoch))
+        filterAttestations(ax, get_block_root(state, epoch))
     }
 
     function method get_attesting_balance(state: BeaconState, attestations: seq<PendingAttestation>) : Gwei 
@@ -276,16 +276,16 @@ module AttestationsHelpers {
      *  @param  br  A root value (hash of a block or block root). 
      *  @returns    The subset of `xl` that corresponds to attestation with target `r`.
      */
-    function method filterAttestationsxx(xl : seq<PendingAttestation>, br : Root) : seq<PendingAttestation>
-        ensures |filterAttestationsxx(xl, br)| <= |xl|
-        ensures forall a :: a in xl && a.data.target.root == br <==> a in filterAttestationsxx(xl, br) 
+    function method filterAttestations(xl : seq<PendingAttestation>, br : Root) : seq<PendingAttestation>
+        ensures |filterAttestations(xl, br)| <= |xl|
+        ensures forall a :: a in xl && a.data.target.root == br <==> a in filterAttestations(xl, br) 
         decreases xl
     {
         if |xl| == 0 then 
             []
         else 
             (if xl[0].data.target.root == br then [xl[0]] else [])
-                + filterAttestationsxx(xl[1..], br)
+                + filterAttestations(xl[1..], br)
     }
    
 }
